src/lib/kuiper/Kuiper.Array.fsti
@@ -15,7 +15,7 @@ open Kuiper.Seq.Common
 module SZ = FStar.SizeT
 
 new
-val gpu_array (a : Type u#0) (sz : nat) : Type u#0
+val gpu_array (a : Type u#0) (sz : SZ.t) : Type u#0
 
 (* FIXME: I think having nat here, which forces to use erased nat
    in concrete functions, hurts Pulse inference a lot. Try to make all
@@ -24,36 +24,36 @@ val gpu_array (a : Type u#0) (sz : nat) : Type u#0
 (* x is the base pointer, this gives permission in [i,j) *)
 val gpu_pts_to_slice
   (#a:Type u#0)
-  (#sz:nat)
+  (#sz:SZ.t)
   ([@@@mkey] x:gpu_array a sz)
   (#[exact (`1.0R)] f : perm)
-  ([@@@mkey] i : nat)
-  (j : nat)
+  ([@@@mkey] i : SZ.t)
+  (j : SZ.t)
   (v : seq a)
 : slprop
 
 unfold
 let gpu_pts_to_cell
   (#a:Type u#0)
-  (#sz:nat)
+  (#sz:SZ.t)
   ([@@@mkey] x:gpu_array a sz)
   (#[exact (`1.0R)] f : perm)
-  ([@@@mkey] i : nat)
+  ([@@@mkey] i : SZ.t{SZ.fits (SZ.v i + 1)})
   (v : a)
 : slprop
 =
-  gpu_pts_to_slice x #f i (i + 1) seq![v]
+  gpu_pts_to_slice x #f i (i `SZ.add` 1sz) seq![v]
 
 unfold
 let gpu_pts_to_array
   (#a:Type u#0)
-  (#sz:nat)
+  (#sz:SZ.t)
   ([@@@mkey] x:gpu_array a sz)
   (#[exact (`1.0R)] f : perm)
   (v : seq a)
 : slprop
 =
-  gpu_pts_to_slice x #f 0 sz v
+  gpu_pts_to_slice x #f 0sz sz v
 
 unfold
 instance has_pts_to_gpu_arr (a:Type) (sz : _) :
@@ -65,10 +65,10 @@ instance has_pts_to_gpu_arr (a:Type) (sz : _) :
 ghost
 fn gpu_pts_to_slice_ref
   (#a:Type u#0)
-  (#sz:nat)
+  (#sz:SZ.t)
   (#f : perm)
   (x:gpu_array a sz)
-  (i:nat) (j:nat)
+  (i:SZ.t) (j:SZ.t)
   (#v : seq a)
   preserves gpu_pts_to_slice x #f i j v
   requires emp
@@ -77,7 +77,7 @@ fn gpu_pts_to_slice_ref
 ghost
 fn gpu_pts_to_ref
   (#a:Type u#0)
-  (#sz:nat)
+  (#sz:SZ.t)
   (#f : perm)
   (x:gpu_array a sz)
   (#v : seq a)
@@ -90,13 +90,13 @@ fn gpu_array_alloc
   {| sized a |}
   (sz : SZ.t)
   preserves cpu
-  returns   x : gpu_array a (SZ.v sz)
+  returns   x : gpu_array a sz
   ensures
     exists* (s:seq a). (x |-> s) ** pure (Seq.length s == sz)
 
 fn gpu_array_free
   (#a:Type u#0)
-  (#sz:erased nat)
+  (#sz:erased SZ.t)
   (r : gpu_array a sz)
   (#v : erased (seq a))
   preserves cpu
@@ -107,43 +107,43 @@ fn gpu_array_free
 atomic
 fn gpu_array_read
   (#a : Type u#0)
-  (#sz : erased nat)
-  (#i  : erased nat)
-  (#j  : erased nat)
+  (#sz : erased SZ.t)
+  (#i  : erased SZ.t)
+  (#j  : erased SZ.t)
   (r:gpu_array a sz)
   (#f:perm)
   (idx : SZ.t)
   (#s : erased (seq a))
   preserves gpu
   preserves gpu_pts_to_slice #a #sz r #f i j s
-  requires pure (i <= SZ.v idx /\ SZ.v idx < j)
+  requires pure (SZ.v i <= SZ.v idx /\ SZ.v idx < SZ.v j)
   returns  x:a
-  ensures  pure (i <= j /\ j <= sz /\ Seq.length s == (j-i) /\
-                 i <= SZ.v idx /\ SZ.v idx < j /\
-                 x == Seq.index s (SZ.v idx - i))
+  ensures  pure (SZ.v i <= SZ.v j /\ SZ.v j <= reveal sz /\ Seq.length s == (SZ.v j - SZ.v i) /\
+                 SZ.v i <= SZ.v idx /\ SZ.v idx < SZ.v j /\
+                 x == Seq.index s (SZ.v idx - SZ.v i))
 
 [@@noextract_to "krml"]
 fn gpu_array_write
   (#a:Type u#0)
-  (#sz: erased nat)
-  (#i: erased nat)
-  (#j: erased nat)
+  (#sz: erased SZ.t)
+  (#i: erased SZ.t)
+  (#j: erased SZ.t)
   (r:gpu_array a sz)
   (idx : SZ.t)
   (v : a)
   (#s : erased (seq a))
   preserves gpu
-  requires pure (i <= SZ.v idx /\ SZ.v idx < j)
+  requires pure (SZ.v i <= SZ.v idx /\ SZ.v idx < SZ.v j)
   requires gpu_pts_to_slice #a #sz r #1.0R i j s
   ensures  (exists* (s':seq a). gpu_pts_to_slice #a #sz r #1.0R i j s' **
-              pure (i <= j /\ j <= sz /\ Seq.length s == (j-i) /\
-                    i <= SZ.v idx /\ SZ.v idx < j /\
-                    s' == Seq.upd s (SZ.v idx - i) v))
+              pure (SZ.v i <= SZ.v j /\ SZ.v j <= reveal sz /\ Seq.length s == (SZ.v j - SZ.v i) /\
+                    SZ.v i <= SZ.v idx /\ SZ.v idx < SZ.v j /\
+                    s' == Seq.upd s (SZ.v idx - SZ.v i) v))
 
 fn gpu_memcpy_host_to_device
   (#a:Type u#0)
   {| sized a |}
-  (#sz : erased nat)
+  (#sz : erased SZ.t)
   (dst_garr : gpu_array a sz)
   (src_arr : vec a)
   (cnt : SZ.t)
@@ -155,192 +155,192 @@ fn gpu_memcpy_host_to_device
     (src_arr |-> Frac f v)
   requires
     (dst_garr |-> gv) **
-    pure (SZ.v cnt == sz /\ (Pulse.Lib.Vec.length src_arr == sz \/ Seq.length v == reveal sz))
+    pure (cnt == sz /\ (Pulse.Lib.Vec.length src_arr == SZ.v sz \/ Seq.length v == reveal sz))
   ensures
     (dst_garr |-> v) **
     pure (Seq.length v == reveal sz)
 
 (* blit *)
-fn gpu_memcpy_host_to_device'
-  (#a:Type u#0)
-  {| sized a |}
-  (#dst_sz : erased nat)
-  (dst_garr : gpu_array a dst_sz)
-  (dst_off : SZ.t)
-  (#src_sz : erased nat)
-  (src_arr : vec a)
-  (src_off : SZ.t)
-  (cnt : SZ.t {
-    dst_off + cnt <= dst_sz /\
-          src_off + cnt <= src_sz
+// fn gpu_memcpy_host_to_device'
+//   (#a:Type u#0)
+//   {| sized a |}
+//   (#dst_sz : erased nat)
+//   (dst_garr : gpu_array a dst_sz)
+//   (dst_off : SZ.t)
+//   (#src_sz : erased nat)
+//   (src_arr : vec a)
+//   (src_off : SZ.t)
+//   (cnt : SZ.t {
+//     dst_off + cnt <= dst_sz /\
+//           src_off + cnt <= src_sz
 
-  })
-  (#f : perm)
-  (#v : erased (seq a){ Seq.length v == src_sz })
-  (#gv : erased (seq a){ Seq.length gv == dst_sz })
-  preserves
-    cpu **
-    pts_to src_arr #f v
-  requires
-    (dst_garr |-> gv)
-  ensures
-    (dst_garr |-> seq_blit gv dst_off v src_off cnt) **
-    pure (Seq.length v == reveal dst_sz)
+//   })
+//   (#f : perm)
+//   (#v : erased (seq a){ Seq.length v == src_sz })
+//   (#gv : erased (seq a){ Seq.length gv == dst_sz })
+//   preserves
+//     cpu **
+//     pts_to src_arr #f v
+//   requires
+//     (dst_garr |-> gv)
+//   ensures
+//     (dst_garr |-> seq_blit gv dst_off v src_off cnt) **
+//     pure (Seq.length v == reveal dst_sz)
 
-fn gpu_memcpy_device_to_host
-  (#a:Type u#0)
-  {| sized a |}
-  (#sz : erased nat)
-  (dst_arr : vec a)
-  (src_garr : gpu_array a sz)
-  (cnt : SZ.t)
-  (#f : perm)
-  (#v : erased (seq a))
-  (#gv : erased (seq a))
-  preserves
-    cpu **
-    (src_garr |-> Frac f gv)
-  requires
-    (dst_arr |-> v) **
-    pure (SZ.v cnt == sz /\ (Pulse.Lib.Vec.length dst_arr == sz \/ Seq.length v == reveal sz))
-  ensures
-    (dst_arr |-> gv) **
-    pure (Seq.length gv == reveal sz)
+// fn gpu_memcpy_device_to_host
+//   (#a:Type u#0)
+//   {| sized a |}
+//   (#sz : erased nat)
+//   (dst_arr : vec a)
+//   (src_garr : gpu_array a sz)
+//   (cnt : SZ.t)
+//   (#f : perm)
+//   (#v : erased (seq a))
+//   (#gv : erased (seq a))
+//   preserves
+//     cpu **
+//     (src_garr |-> Frac f gv)
+//   requires
+//     (dst_arr |-> v) **
+//     pure (SZ.v cnt == sz /\ (Pulse.Lib.Vec.length dst_arr == sz \/ Seq.length v == reveal sz))
+//   ensures
+//     (dst_arr |-> gv) **
+//     pure (Seq.length gv == reveal sz)
 
-(* blit *)
-fn gpu_memcpy_device_to_host'
-  (#a:Type u#0)
-  {| sized a |}
-  (#dst_sz : erased nat)
-  (dst_arr : vec a)
-  (dst_off : SZ.t)
-  (#src_sz : erased nat)
-  (src_garr : gpu_array a src_sz)
-  (src_off : SZ.t)
-  (cnt : SZ.t {
-    dst_off + cnt <= dst_sz /\
-          src_off + cnt <= src_sz
-  })
-  (#f : perm)
-  (#v : erased (seq a){ Seq.length v == src_sz })
-  (#gv : erased (seq a){ Seq.length gv == dst_sz })
-  preserves
-    cpu **
-    pts_to src_garr #f v
-  requires
-    (dst_arr |-> gv)
-  ensures
-    (dst_arr |-> seq_blit gv dst_off v src_off cnt) **
-    pure (Seq.length v == reveal dst_sz)
+// (* blit *)
+// fn gpu_memcpy_device_to_host'
+//   (#a:Type u#0)
+//   {| sized a |}
+//   (#dst_sz : erased nat)
+//   (dst_arr : vec a)
+//   (dst_off : SZ.t)
+//   (#src_sz : erased nat)
+//   (src_garr : gpu_array a src_sz)
+//   (src_off : SZ.t)
+//   (cnt : SZ.t {
+//     dst_off + cnt <= dst_sz /\
+//           src_off + cnt <= src_sz
+//   })
+//   (#f : perm)
+//   (#v : erased (seq a){ Seq.length v == src_sz })
+//   (#gv : erased (seq a){ Seq.length gv == dst_sz })
+//   preserves
+//     cpu **
+//     pts_to src_garr #f v
+//   requires
+//     (dst_arr |-> gv)
+//   ensures
+//     (dst_arr |-> seq_blit gv dst_off v src_off cnt) **
+//     pure (Seq.length v == reveal dst_sz)
 
-fn gpu_memcpy_device_to_device
-  (#a:Type u#0)
-  {| sized a |}
-  (#sz : erased nat)
-  (dst_arr : gpu_array a sz)
-  (src_garr : gpu_array a sz)
-  (cnt : SZ.t)
-  (#f : perm)
-  (#v : erased (seq a))
-  (#gv : erased (seq a))
-  preserves
-    cpu **
-    (src_garr |-> Frac f gv)
-  requires
-    (dst_arr |-> v) **
-    pure (SZ.v cnt == sz /\ (Seq.length gv == sz \/ Seq.length v == sz))
-  ensures
-    (dst_arr |-> gv) **
-    pure (Seq.length gv == reveal sz)
+// fn gpu_memcpy_device_to_device
+//   (#a:Type u#0)
+//   {| sized a |}
+//   (#sz : erased nat)
+//   (dst_arr : gpu_array a sz)
+//   (src_garr : gpu_array a sz)
+//   (cnt : SZ.t)
+//   (#f : perm)
+//   (#v : erased (seq a))
+//   (#gv : erased (seq a))
+//   preserves
+//     cpu **
+//     (src_garr |-> Frac f gv)
+//   requires
+//     (dst_arr |-> v) **
+//     pure (SZ.v cnt == sz /\ (Seq.length gv == sz \/ Seq.length v == sz))
+//   ensures
+//     (dst_arr |-> gv) **
+//     pure (Seq.length gv == reveal sz)
 
 
 (* Not making this unfold as it appears under bigstars. Maybe
 pulse should only do weak unfolding. *)
 let gpu_pts_to_array1
   (#a:Type0)
-  (#sz:nat)
+  (#sz:SZ.t)
   ([@@@mkey]arr : gpu_array a sz)
   (#[exact (`1.0R)] f : perm)
-  ([@@@mkey]i:nat)
+  ([@@@mkey]i:SZ.t{SZ.fits (SZ.v i + 1)})
 : slprop =
-  exists* s. gpu_pts_to_slice arr i (i+1) s
+  exists* s. gpu_pts_to_slice arr i (i `SZ.add` 1sz) s
 
 ghost
 fn gpu_array_slice_1
   (#[exact (`0)] uid: int) (#a:Type u#0)
-  (#sz:nat)
+  (#sz:SZ.t)
   (arr : gpu_array a sz)
   (#f : perm)
   (#v : erased (seq a) { Seq.length v == sz })
   requires pts_to arr #f v
-  ensures  bigstar #uid 0 sz (fun i -> gpu_pts_to_slice arr #f i (i+1) seq![v @! i])
+  ensures  bigstar #uid 0 sz (fun i -> gpu_pts_to_slice arr #f (SZ.uint_to_t i) (SZ.uint_to_t (i+1)) seq![v @! i])
 
 ghost
 fn gpu_array_unslice_1
   (#uid: int) (#a:Type u#0)
-  (#sz:nat)
+  (#sz:SZ.t)
   (arr : gpu_array a sz)
   (#f : perm)
   (#v : erased (seq a) { Seq.length v == sz })
-  requires bigstar #uid 0 sz (fun i -> gpu_pts_to_slice arr #f i (i+1) seq![v @! i])
+  requires bigstar #uid 0 sz (fun i -> gpu_pts_to_slice arr #f (SZ.uint_to_t i) (SZ.uint_to_t (i+1)) seq![v @! i])
   ensures  pts_to arr #f v
 
 ghost
 fn gpu_array_slice_1_underspec
   (#[exact (`0)] uid: int) (#a:Type u#0)
-  (#sz:nat)
+  (#sz:SZ.t)
   (arr : gpu_array a sz)
   (#f : perm)
   (#v : erased (seq a))
   requires arr |-> Frac f v
-  ensures  bigstar #uid 0 sz (gpu_pts_to_array1 arr #f)
+  ensures  bigstar #uid 0 sz (fun i -> gpu_pts_to_array1 arr #f (SZ.uint_to_t i))
 
 ghost
 fn gpu_array_unslice_1_underspec
   (#uid: int) (#a:Type u#0)
-  (#sz:nat)
+  (#sz:SZ.t)
   (arr : gpu_array a sz)
   (#f : perm)
-  requires bigstar #uid 0 sz (gpu_pts_to_array1 arr #f)
+  requires bigstar #uid 0 sz (fun i -> gpu_pts_to_array1 arr #f (SZ.uint_to_t i))
   ensures exists* (v : seq a). arr |-> Frac f v
 
 ghost
 fn gpu_slice_concat
   (#a:Type u#0)
-  (#sz:nat)
+  (#sz:SZ.t)
   (arr : gpu_array a sz)
   (#[exact (`1.0R)] f : perm)
   (#s1 #s2: erased (seq a))
-  (i n m:nat)
+  (i n m:SZ.t)
   requires gpu_pts_to_slice arr #f i n s1 ** gpu_pts_to_slice arr #f n m s2
   ensures  gpu_pts_to_slice arr #f i m (Seq.append s1 s2)
 
 ghost
 fn gpu_slice_split
   (#a:Type u#0)
-  (#sz:nat)
+  (#sz:SZ.t)
   (arr : gpu_array a sz)
   (#[exact (`1.0R)] f : perm)
   (#s1 #s2: erased (seq a))
-  (i n m:nat)
+  (i n m:SZ.t)
   requires gpu_pts_to_slice arr #f i m (Seq.append s1 s2)
   ensures  gpu_pts_to_slice arr #f i n s1 ** gpu_pts_to_slice arr #f n m s2
 
 ghost
 fn gpu_slice_empty_elim
-  (#a:Type u#0) (#sz:nat)
+  (#a:Type u#0) (#sz:SZ.t)
   (arr : gpu_array a sz)
-  (i : nat)
+  (i : SZ.t)
   requires gpu_pts_to_slice arr #'f i i 'v
   ensures  emp
 
 ghost
 fn gpu_slice_share
   (#uid: int) (#a:Type u#0)
-  (#sz:nat)
+  (#sz:SZ.t)
   (arr : gpu_array a sz)
-  (m n:nat)
-  (k: nat { k > 0 })
+  (m n:SZ.t)
+  (k: SZ.t { k > 0 })
   (#f : perm)
   requires gpu_pts_to_slice arr #f m n 'v
   ensures
@@ -349,10 +349,10 @@ fn gpu_slice_share
 ghost
 fn gpu_slice_gather
   (#uid: int) (#a:Type u#0)
-  (#sz:nat)
+  (#sz:SZ.t)
   (arr : gpu_array a sz)
-  (m n:nat)
-  (k: nat { k > 0 })
+  (m n:SZ.t)
+  (k: SZ.t { k > 0 })
   (#f : perm) // FIXME: if we use 'f, it gets type 'real' instead of 'perm'
   requires
     bigstar #uid 0 k (fun _ -> gpu_pts_to_slice arr #(f /. Real.of_int k) m n 'v)
@@ -361,21 +361,21 @@ fn gpu_slice_gather
 ghost
 fn gpu_slice_share_underspec
   (#uid : int) (#a : Type u#0)
-  (#sz : nat)
+  (#sz : SZ.t)
   (arr : gpu_array a sz)
-  (m n : nat)
-  (k : nat { k > 0 })
+  (m n : SZ.t)
+  (k : SZ.t { k > 0 })
   requires gpu_pts_to_slice arr #'f m n 'v
   ensures bigstar #uid 0 k (fun x -> exists* v. gpu_pts_to_slice arr #('f /. Real.of_int k) m n v)
 
 ghost
 fn gpu_slice_gather_underspec
   (#uid : int) (#a : Type u#0)
-  (#sz : nat)
+  (#sz : SZ.t)
   (arr : gpu_array a sz)
   (#f : perm) // FIXME: if we use 'f, it gets type 'real' instead of 'perm'
-  (m n : nat)
-  (k : nat { k > 0 })
+  (m n : SZ.t)
+  (k : SZ.t { k > 0 })
   requires bigstar #uid 0 k (fun x -> exists* v. gpu_pts_to_slice arr #(f /. Real.of_int k) m n v)
   ensures
     exists* v.
@@ -383,7 +383,7 @@ fn gpu_slice_gather_underspec
 
 val adjacent
   (#a : Type u#0)
-  (#s1 #s2 : nat)
+  (#s1 #s2 : SZ.t)
   (arr1 : gpu_array a s1)
   (arr2 : gpu_array a s2)
   : slprop
@@ -391,7 +391,7 @@ val adjacent
 ghost
 fn gpu_array_cut
   (#a : Type u#0)
-  (#sz : nat)
+  (#sz : SZ.t)
   (arr : gpu_array a sz)
   (#f : perm) // FIXME: if we use 'f, it gets type 'real' instead of 'perm'
   (k : SZ.t{ k <= sz })
@@ -399,7 +399,7 @@ fn gpu_array_cut
   requires
     (arr |-> Frac f s)
   returns
-    p : (gpu_array a k & gpu_array a (sz - k))
+    p : (gpu_array a k & gpu_array a (sz `SZ.sub` k))
   ensures
     (p._1 |-> Frac f (seq_take k s)) **
     (p._2 |-> Frac f (seq_drop k s)) **
@@ -408,7 +408,7 @@ fn gpu_array_cut
 ghost
 fn gpu_array_paste
   (#a : Type u#0)
-  (#sz1 #sz2 : nat)
+  (#sz1 #sz2 : SZ.t {SZ.fits (SZ.v sz1 + SZ.v sz2)})
   (arr1 : gpu_array a sz1)
   (arr2 : gpu_array a sz2)
   (#f : perm)
@@ -417,6 +417,6 @@ fn gpu_array_paste
     (arr2 |-> Frac f 's2) **
     adjacent arr1 arr2
   returns
-    arr : gpu_array a (sz1 + sz2)
+    arr : gpu_array a (sz1 `SZ.add` sz2)
   ensures
     arr |-> Frac f (Seq.append 's1 's2)
